\documentclass{alittlebear}
\def\filenum{1}
\pagestyle{style}

\begin{document}

\begin{exercise}{}{}
    \begin{note}
        This exercise aims at computing the following indefinite integral

        $$J_{n}=\int \frac{1}{\left(x^{2}+a^{2}\right)^{n}}\D x, n \in \mathbb{N}$$
    \end{note}

    \begin{question}{}{}
        Compute $J_{1}$.
        \tcblower

        \begin{mathnote}
            \begin{align*}
                J_1&=\int \frac{\D x}{x^2+a^2}\\
                &=\int \frac1{a^2}\cdot\frac{\D x}{(\frac{x}a)^2+1}\\
                &=\frac1a \int \frac{\D (\frac{x}a)}{(\frac{x}a)^2+1}\\
                &=\frac1a\arctan(\frac{x}a)+C
            \end{align*}
        \end{mathnote}
    \end{question}

    \begin{question}{}{}
        Compute $J_{2}$.
        \begin{hint}
            Consider the substitution $x=\tan t$.
        \end{hint}
        \tcblower
        \begin{mathnote}
            \begin{align*}
                J_2 &=\int \frac{\D x}{(x^2+a^2)^2}\\
                \text{Substitute } x&=\tan t\\
                \D x&=\sec^2 t \cdot \D t\\
                J_2&=\int \frac{\sec^2 t}{(\tan^2 t + a^2)^2}\D t\\
                \D (\frac{1}{\tan^2 t + a^2}) &= -\frac{2\tan t\sec^2 t}{(\tan^2 t + a^2)^2}\D t\\
                J_2&=-\int \frac{1}{2\tan t}\D (\frac{1}{\tan^2 t + a^2})\\
                &=-\int \frac{1}{2x}\D (\frac{1}{x^2+a^2})\\
                \text{By integration by parts, we have }&\\
                J_2&=-\frac{1}{2x(x^2+a^2)}+\int \frac{1}{x^2+a^2}\D (\frac{1}{2x})\\
                &=-\frac{1}{2x(x^2+a^2)}+\frac{1}{2}\int \frac{1}{x^2+a^2}\D (\frac{1}{x})\\
                &=-\frac{1}{2x(x^2+a^2)}-\frac{1}{2}\int \frac{1}{x^2+a^2}\frac{1}{x^2}\D x\\
                \text{By partial fractions, we have}\\
                J_2&=-\frac{1}{2x(x^2+a^2)}-\frac{1}{2}\int -\frac{1}{a^2(x^2+a^2)}+\frac{1}{a^2x^2}\D x\\
                &=-\frac{1}{2x(x^2+a^2)}+\frac{1}{2}\int \frac{1}{a^2(x^2+a^2)}\D x -\frac{1}{2}\int\frac{1}{a^2x^2}\D x\\
                &=-\frac{1}{2x(x^2+a^2)}+\frac{1}{2a^2}\int \frac{1}{x^2+a^2}\D x -\frac{1}{2a^2}\int\frac{1}{x^2}\D x\\
                &=-\frac{1}{2x(x^2+a^2)}+\frac{1}{2a^3}\arctan(\frac{x}a) +\frac{1}{2a^2 x} + C\\
                &=\frac{x^2+a^2-a^2}{2xa^2(x^2+a^2)}+\frac{1}{2a^3}\arctan(\frac{x}a) + C\\
                &=\frac{x}{2a^2(x^2+a^2)}+\frac{1}{2a^3}\arctan(\frac{x}a) + C\\
            \end{align*}
        \end{mathnote}
    \end{question}

    \begin{question}{}{}
        Prove that $\forall n \in \mathbb{N}$, $$
        J_{n}=\frac{x}{\left(x^{2}+a^{2}\right)^{n}}+2 n \int \frac{x^{2}}{\left(x^{2}+a^{2}\right)^{n+1}} d x
        $$

        \begin{hint}
            Consider integration by parts.
        \end{hint}

        \begin{proof}{}{}
            Pick an arbitrary $n\in\N$, we have that
            \begin{align*}
            \D (\frac{1}{(x^2+a^2)^{n}}) &= -\frac{2nx}{(x^2+a^2)^{n+1}}\D x\\
                \frac{x}{(x^2+a^2)^{n}}+2n\int \frac{x^2}{(x^2+a^2)^{n+1}}\D x &= \frac{x}{(x^2+a^2)^{n}}+2n\int -\frac{x}{2n}\D (\frac{1}{(x^2+a^2)^{n}})\\
                &=\frac{x}{(x^2+a^2)^{n}}-\int x\D (\frac{1}{(x^2+a^2)^{n}})\\
                \text{By integration by parts, }\\
                \frac{x}{(x^2+a^2)^{n}}-\int x\D (\frac{1}{(x^2+a^2)^{n}}) &= \frac{x}{(x^2+a^2)^{n}} - \frac{x}{(x^2+a^2)^{n}} + \int \frac{1}{(x^2+a^2)^{n}}\D x\\
                &= \int \frac{1}{(x^2+a^2)^{n}}\D x\\
                &= J_n
            \end{align*}
            Thus we have shown for any $n\in\N$ the equality holds, completing our proof.
        \end{proof}
    \end{question}

    \begin{question}{}{}
        Based on the previous sub-question, establish the recursive relation:

        $$
        J_{n+1}=\frac{2 n-1}{2 n} \frac{1}{a^{2}} J_{n}+\frac{1}{2 n a^{2}} \frac{x}{\left(x^{2}+a^{2}\right)^{n}}
        $$

        From there, conclude that $J_{n}$ is an integral of finite terms (i.e., it is an elementary function) 

        \tcblower

        \begin{mathnote}
            \begin{align*}
                J_{n+1}&=\int \frac{1}{(x^2+a^2)^{n+1}}\D x\\
                &= \frac1{a^2}\int \frac{(x^2+a^2)-x^2}{(x^2+a^2)^{n+1}}\D x\\
                &=\frac1{a^2}\int\frac1{(x^2+a^2)^n}\D x - \frac1{a^2}\int\frac{x^2}{(x^2+a^2)^{n+1}}\D x\\
                &=\frac1{a^2}J_n - \frac1{a^2}\int -\frac{x}{2n}\D (\frac{1}{(x^2+a^2)^n})\\
                &=\frac1{a^2}J_n + \frac1{2na^2}\int x\D (\frac{1}{(x^2+a^2)^n})\\
                &=\frac1{a^2}J_n + \frac{1}{2na^2}\left[\frac{x}{(x^2+a^2)^n}-\int\frac1{(x^2+a^2)^n}\D x \right]\\
                &=\frac1{a^2}J_n + \frac1{2na^2}\frac{x}{(x^2+a^2)^n}-\frac{1}{2na^2}J_n\\
                &=J_n[\frac{1}{a^2}-\frac{1}{2na^2}]+\frac{1}{2na^2}\frac{x}{(x^2+a^2)^n}\\
                &=(1-\frac1{2n})\frac1{a^2}J_n + \frac1{2na^2}\frac{x}{(x^2+a^2)^n}\\
                &=\frac{2n-1}{2n}\frac1{a^2}J_n + \frac1{2na^2}\frac{x}{(x^2+a^2)^n}
            \end{align*}

            as needed.
        \end{mathnote}

    \end{question}

    \begin{question}{}{}
        Compute $J_{3}$.
        \tcblower
        \begin{mathnote}
            By Q4's formula, combining with our result of $J_2$, we have that

            \begin{align*}
                J_3&=\frac{4-1}{4}\frac{1}{a^2}J_2+\frac{1}{4a^2}\frac{x}{(x^2+a^2)^2}\\
                &=\frac{4-1}{4}\frac{1}{a^2}[\frac{x}{2a^2(x^2+a^2)}+\frac{1}{2a^3}\arctan(\frac{x}a) + C]+\frac{1}{4a^2}\frac{x}{(x^2+a^2)^2}\\
                &=\frac{3}{4a^2}\frac{x}{2a^2(x^2+a^2)}+\frac{3}{4a^2}\frac{1}{2a^3}\arctan(\frac{x}a)+\frac{1}{4a^2}\frac{x}{(x^2+a^2)^2} + C\\
                &=\frac{1}{4a^2}\left[\frac{3}{2a^3}\arctan(\frac{x}a)+\frac{3x}{2a^2(x^2+a^2)}+\frac{x}{(x^2+a^2)^2}\right] + C\\
            \end{align*}
        \end{mathnote}
    \end{question}
\end{exercise}

\end{document}